Add trail

cfrontend/MoSel.v
@@ -100,36 +100,40 @@ Module gensym.
   Export SepList.
 
   Definition ident := positive.
-  (* =generator= *)
+(* =generator= *)
 Record generator : Type := mkgenerator { gen_next : ident;
                                          gen_trail: list (ident * type)
                                        }.
 
 Definition initial_state : generator := mkgenerator 1%positive nil.
-  (* =end= *)
-  (* =mon= *)
+(* =end= *)
+(* =mon= *)
 Inductive mon (X : Type) : Type :=
 | ret : X -> mon X
 | errorOp : Errors.errmsg -> mon X
-| gensymOp : type -> (ident -> mon X) -> mon X.
-  (* =end= *)
+| gensymOp : type -> (ident -> mon X) -> mon X
+| trailOp : (list (ident * type) -> mon X) -> mon X.
+(* =end= *)
   Arguments errorOp [X].
   Arguments gensymOp [X].
+  Arguments trailOp [X].
   Arguments ret {_} x.
-  (* =bind= *)
+(* =bind= *)
 Fixpoint bind {X Y} (m : mon X) (f : X -> mon Y) : mon Y :=
   match m with
   | ret x => f x
   | errorOp e => errorOp e
   | gensymOp t g => gensymOp t (fun x => bind (g x) f)
+  | trailOp g => trailOp (fun x => bind (g x) f)
   end.
-  (* =end= *)
+(* =end= *)
   Notation "'let!' x ':=' e1 'in' e2" := (bind e1 (fun x => e2)) (x ident, at level 90).
 
   Notation "'ret!' v" := (ret v) (v ident, at level 90).
-  (* =operators= *)
+(* =operators= *)
 Definition error {X} (e : Errors.errmsg) : mon X := errorOp e.
 Definition gensym (t : type) : mon ident := gensymOp t ret.
+Definition trail : mon (list (ident * type)) := trailOp ret.
 (* =end= *)
   Lemma lid : forall X Y (a : X) (f : X -> mon Y), bind (ret a) f = f a.
   Proof. auto. Qed.
@@ -138,9 +142,8 @@ Definition gensym (t : type) : mon ident := gensymOp t ret.
   Proof.
     fix m 2.
     destruct m0.
-    * reflexivity.
-    * reflexivity.
-    * simpl. do 2 f_equal. apply functional_extensionality. intro. apply m.
+    1 - 2 : reflexivity.
+    all : simpl; do 2 f_equal; apply functional_extensionality; intro; apply m.
   Qed.
 
   Lemma ass_bind : forall X Y Z (m : mon X) f (g : Y -> mon Z),
@@ -148,9 +151,8 @@ Definition gensym (t : type) : mon ident := gensymOp t ret.
   Proof.
     fix m 4.
     destruct m0; intros.
-    * reflexivity.
-    * reflexivity.
-    * simpl. do 2 f_equal. apply functional_extensionality. intro. apply m.
+    1 - 2 : reflexivity.
+    all : simpl; do 2 f_equal; apply functional_extensionality; intro; apply m.
   Qed.
 
 (* =eval= *)
@@ -163,6 +165,10 @@ Fixpoint eval {X} (m : mon X) : generator -> res (generator * X) :=
       let h := gen_trail s in
       let n := gen_next s in
       eval (f n) (mkgenerator (Pos.succ n) ((n,ty) :: h))
+  | trailOp f =>
+    fun s =>
+      let h := gen_trail s in
+      eval (f h) s
   end.
 (* =end= *)
 
@@ -189,6 +195,7 @@ Fixpoint wp {X} (e1 : mon X) (Q : X -> iProp) : iProp :=
   | ret v => Q v
   | errorOp e => True
   | gensymOp _ f => ∀ l, IsFresh l -∗ wp (f l) Q
+  | trailOp f => ∀ l, wp (f l) Q
   end.
 (* =end= *)
   Notation "'{{' P } } e {{ v ; Q } }" := (P -∗ wp e (fun v => Q))
@@ -204,9 +211,8 @@ Proof.
   destruct e0.
   - iApply "HB". iApply "HA".
   - simpl. auto.
-  - simpl. iIntros (l) "HC".
-      iDestruct ("HA" with "HC") as "HA".
-      iPoseProof "HB" as "HB". apply e.
+  - simpl. iIntros (l) "HC". iDestruct ("HA" with "HC") as "HA". iPoseProof "HB" as "HB". apply e.
+  - simpl. iIntros (l). iDestruct ("HA" $! l) as "HA". iPoseProof "HB" as "HB". apply e.
 Qed.
 
 Lemma wp_consequence : forall {X} (P Q : X -> iProp) (f : mon X),
@@ -217,6 +223,7 @@ Proof.
   induction f; simpl; intros; auto.
   - iIntros "HA HB". iApply ("HB" with "HA").
   - iIntros "HA * HB * HC". iApply (H with "[HA HC] HB"). iApply ("HA" with "HC").
+  - iIntros "HA HB *". iApply (H with "HA HB").
 Qed.
 
 Lemma ret_spec {X} (v : X) H (Q : X -> iProp) :
@@ -284,6 +291,12 @@ Lemma error_spec {X} (Q : X -> iProp) e : ⊢{{ True }} error e {{ v; Q v }}.
 (* =end= *)
 Proof. auto. Qed.
 
+
+(* =trail_spec= *)
+Lemma trail_spec : ⊢{{ emp }} trail {{ _; emp  }}.
+(* =end= *)
+Proof. auto. Qed.
+
 End weakestpre_gensym.
 
 Module adequacy.
@@ -327,6 +340,7 @@ Module adequacy.
         iDestruct (heap_ctx_split with "HA") as "[HA HB]". apply next_disjoint.
         iDestruct (H with "HA") as "HA".
         iApply ("HA" with "HB").
+    - simpl in *. eapply e; eauto. iIntros "HA". iApply (H with "HA").
   Qed.
 
   Lemma adequacy_init {X} : forall (e : mon X) (Q : X -> iProp) s' v,
@@ -379,19 +393,20 @@ Lemma adequacy_core {X} : forall (e : mon X) (Q : X -> iProp) s v s' H,
   Implicit Type Q: X -> Prop.
   Implicit Type v: X.
 
-(* =adequacy= *)
-Lemma adequacy: forall m P Q v,
-   (⊢ P) -> (⊢ {{ P }} m {{ v; ⌜ Q v ⌝}}) ->
-   run m = OK v -> Q v.
-(* =end= *)
+  (* =adequacy_pure= *)
+  Lemma adequacy: forall m Q v,
+      (⊢ {{ emp }} m {{ v; ⌜ Q v ⌝}}) ->
+      run m = OK v -> Q v.
+  (* =end= *)
   Proof.
   intros m.
   unfold run. intros.
-  destruct (eval m initial_state) eqn:H2; try inversion H1.
-  destruct p. inversion H1; subst.
+  destruct (eval m initial_state) eqn:H2.
+  destruct p. inversion H0. subst.
   eapply adequacy_pure; eauto.
   iIntros "_".
-  iApply H0. iApply H.
+  iApply H. auto.
+  inversion H0.
   Qed.
 
   End Adequacy.
